Refactoring low-level Merkle tree; wip building Vector and BufVector libraries

examples/low-level/merkletree/LowStar.Vector.fst
@@ -7,58 +7,136 @@ open LowStar.Modifies
 module HS = FStar.HyperStack
 module HST = FStar.HyperStack.ST
 module B = LowStar.Buffer
+module S = FStar.Seq
 
 type uint32_t = UInt32.t
 
 val max_uint32: uint32_t
 let max_uint32 = UInt32.uint_to_t (UInt.max_int UInt32.n)
 
-let root = Monotonic.HyperHeap.root
+module U32 = FStar.UInt32
 
 /// Abstract vector type
 
 noeq type vector_str a =
-| Vec: sz:uint32_t{sz > 0ul} ->
-       cap:uint32_t{cap >= sz} ->
+| Vec: sz:uint32_t ->
+       cap:uint32_t{cap > 0ul && cap >= sz} ->
        vs:B.buffer a{B.len vs = cap} -> 
        vector_str a
 
 val vector (a: Type0): Tot Type0
 let vector a = vector_str a
 
-/// Construction
+/// Specification
 
-val create: 
-  #a:Type -> len:uint32_t{len > 0ul} -> a -> 
-  HST.ST (vector a)
-	 (requires (fun h0 -> true))
-	 (ensures (fun h0 vec h1 -> modifies loc_none h0 h1))
-let create #a n v =
-  Vec n n (B.malloc root v n)
+val as_seq: HS.mem -> #a:Type -> vec:vector a -> GTot (S.seq a)
+let as_seq h #a vec =
+  B.as_seq h (B.gsub (Vec?.vs vec) 0ul (Vec?.sz vec))
 
-/// Heap conditions
+/// Memory-related
 
-val live: #a:Type -> HS.mem -> vector a -> GTot Type0
-let live #a h vec =
+unfold val live: #a:Type -> HS.mem -> vector a -> GTot Type0
+unfold let live #a h vec =
   B.live h (Vec?.vs vec)
+
+unfold val freeable: #a:Type -> vector a -> GTot Type0
+unfold let freeable #a vec =
+  B.freeable (Vec?.vs vec)
+
+unfold val loc_vector: #a:Type -> vector a -> GTot loc
+unfold let loc_vector #a vec =
+  B.loc_buffer (Vec?.vs vec)
+
+unfold val loc_addr_of_vector: #a:Type -> vector a -> GTot loc
+unfold let loc_addr_of_vector #a vec =
+  B.loc_addr_of_buffer (Vec?.vs vec)
+
+unfold val frameOf: #a:Type -> vector a -> GTot Monotonic.HyperHeap.rid
+unfold let frameOf #a vec =
+  B.frameOf (Vec?.vs vec)
 
 /// Capacity
 
-val size_of: #a:Type -> vec:vector a -> Tot uint32_t
-let size_of #a vec = 
+unfold val size_of: #a:Type -> vec:vector a -> Tot uint32_t
+unfold let size_of #a vec = 
   Vec?.sz vec
 
-val capacity_of: #a:Type -> vec:vector a -> Tot uint32_t
-let capacity_of #a vec =
+unfold val capacity_of: #a:Type -> vec:vector a -> Tot uint32_t
+unfold let capacity_of #a vec =
   Vec?.cap vec
 
-val is_empty: #a:Type -> vec:vector a -> Tot bool
-let is_empty #a vec =
+unfold val is_empty: #a:Type -> vec:vector a -> Tot bool
+unfold let is_empty #a vec =
   size_of vec = 0ul
 
-val is_full: #a:Type -> vstr:vector_str a -> GTot bool
-let is_full #a vstr =
+unfold val is_full: #a:Type -> vstr:vector_str a -> GTot bool
+unfold let is_full #a vstr =
   Vec?.sz vstr >= max_uint32
+
+/// Construction
+
+val create_rid:
+  #a:Type -> len:uint32_t{len > 0ul} -> v:a ->
+  rid:Monotonic.HyperHeap.rid{HST.is_eternal_region rid} ->
+  HST.ST (vector a)
+	 (requires (fun h0 -> true))
+	 (ensures (fun h0 vec h1 -> 
+	   frameOf vec = rid /\ 
+	   live h1 vec /\ freeable vec /\
+	   modifies loc_none h0 h1 /\
+	   size_of vec = len /\
+	   S.equal (as_seq h1 vec) (S.create (U32.v len) v)))
+let create_rid #a len v rid =
+  Vec len len (B.malloc rid v len)
+
+val create: 
+  #a:Type -> len:uint32_t{len > 0ul} -> v:a -> 
+  HST.ST (vector a)
+	 (requires (fun h0 -> true))
+	 (ensures (fun h0 vec h1 -> 
+	   frameOf vec = Monotonic.HyperHeap.root /\
+	   live h1 vec /\ freeable vec /\
+	   modifies loc_none h0 h1 /\
+	   size_of vec = len /\
+	   S.equal (as_seq h1 vec) (S.create (U32.v len) v)))
+let create #a len v =
+  create_rid len v Monotonic.HyperHeap.root
+
+val create_reserve:
+  #a:Type -> len:uint32_t{len > 0ul} -> ia:a ->
+  rid:Monotonic.HyperHeap.rid{HST.is_eternal_region rid} ->
+  HST.ST (vector a)
+	 (requires (fun h0 -> true))
+	 (ensures (fun h0 vec h1 -> 
+	   frameOf vec = rid /\ live h1 vec /\ freeable vec /\
+	   modifies loc_none h0 h1 /\
+	   size_of vec = 0ul /\
+	   S.equal (as_seq h1 vec) S.empty))
+let create_reserve #a len ia rid =
+  Vec 0ul len (B.malloc rid ia len)
+
+val create_by_buffer:
+  #a:Type -> len:uint32_t{len > 0ul} ->
+  buf:B.buffer a{B.len buf = len} ->
+  HST.ST (vector a)
+	 (requires (fun h0 -> B.live h0 buf))
+	 (ensures (fun h0 vec h1 -> 
+	   frameOf vec = B.frameOf buf /\ loc_vector vec == B.loc_buffer buf /\
+	   live h1 vec /\ h0 == h1 /\
+	   size_of vec = len /\
+	   S.equal (as_seq h1 vec) (B.as_seq h0 buf)))
+let create_by_buffer #a len buf =
+  Vec len len buf
+
+/// Destruction
+
+val free:
+  #a:Type -> vec:vector a ->
+  HST.ST unit
+    (requires (fun h0 -> live h0 vec /\ freeable vec))
+    (ensures (fun h0 _ h1 -> modifies (loc_addr_of_vector vec) h0 h1))
+let free #a vec =
+  B.free (Vec?.vs vec)
 
 /// Element access
 
@@ -66,7 +144,9 @@ val index:
   #a:Type -> vec:vector a -> i:uint32_t -> 
   HST.ST a
     (requires (fun h0 -> live h0 vec /\ i < Vec?.sz vec))
-    (ensures (fun h0 _ h1 -> h0 == h1))
+    (ensures (fun h0 v h1 -> 
+      h0 == h1 /\
+      S.index (as_seq h1 vec) (U32.v i) == v))
 let index #a vec i =
   B.index (Vec?.vs vec) i
 
@@ -75,7 +155,9 @@ val assign:
   i:uint32_t -> v:a ->
   HST.ST unit
     (requires (fun h0 -> live h0 vec /\ i < Vec?.sz vec))
-    (ensures (fun h0 _ h1 -> modifies (loc_buffer (Vec?.vs vec)) h0 h1))
+    (ensures (fun h0 _ h1 -> 
+      modifies (loc_buffer (Vec?.vs vec)) h0 h1 /\
+      S.equal (as_seq h1 vec) (S.upd (as_seq h0 vec) (U32.v i) v)))
 let assign #a vec i v =
   B.upd (Vec?.vs vec) i v
 
@@ -84,7 +166,7 @@ let assign #a vec i v =
 private val resize_ratio: uint32_t
 private let resize_ratio = 2ul
 
-private val new_capacity: uint32_t -> Tot uint32_t
+private val new_capacity: cap:uint32_t{cap > 0ul} -> Tot uint32_t
 private let new_capacity cap =
   if cap >= max_uint32 / resize_ratio then max_uint32
   else cap * resize_ratio
@@ -92,26 +174,143 @@ private let new_capacity cap =
 val insert: 
   #a:Type -> vec:vector a -> v:a -> 
   HST.ST (vector a)
-    (requires (fun h0 ->
-      live h0 vec /\ not (is_full vec)))
+    (requires (fun h0 -> live h0 vec /\ not (is_full vec)))
     (ensures (fun h0 nvec h1 ->
+      live h1 vec /\
       modifies (loc_union (loc_buffer (Vec?.vs vec)) 
 			  (loc_buffer (Vec?.vs nvec))) h0 h1 /\
-      Vec?.sz nvec = Vec?.sz vec + 1ul /\
-      B.as_seq h1 (B.gsub (Vec?.vs nvec) 0ul (Vec?.sz vec)) ==
-      B.as_seq h0 (B.gsub (Vec?.vs vec) 0ul (Vec?.sz vec)) /\
-      B.get h1 (Vec?.vs nvec) (UInt32.v (Vec?.sz vec)) == v))
+      S.equal (as_seq h1 nvec) (S.snoc (as_seq h0 vec) v)))
 let insert #a vec v =
   let sz = Vec?.sz vec in
   let cap = Vec?.cap vec in
   let vs = Vec?.vs vec in
-  if sz = cap then
-    (let ncap = new_capacity cap in
-    let nvs = B.malloc root v ncap in
-    B.blit vs 0ul nvs 0ul sz;
-    B.upd nvs sz v;
-    Vec (sz + 1ul) ncap nvs)
+  if sz = cap 
+  then (let ncap = new_capacity cap in
+       // let nvs = B.malloc (B.frameOf vs) v ncap in
+       let nvs = B.malloc Monotonic.HyperHeap.root v ncap in
+       B.blit vs 0ul nvs 0ul sz;
+       B.upd nvs sz v;
+       // B.free vs; // TODO!
+       Vec (sz + 1ul) ncap nvs)
   else
     (B.upd vs sz v;
     Vec (sz + 1ul) cap vs)
+
+/// Iteration
+
+val fold_left_seq:
+  #a:Type -> #b:Type0 -> seq:S.seq a ->
+  f:(b -> a -> Tot b) -> ib:b -> 
+  GTot b (decreases (S.length seq))
+let rec fold_left_seq #a #b seq f ib =
+  if S.length seq = 0 then ib
+  else fold_left_seq (S.tail seq) f (f ib (S.head seq))
+
+val fold_left_buffer:
+  #a:Type -> #b:Type0 -> len:uint32_t ->
+  buf:B.buffer a{B.len buf = len} ->
+  f:(b -> a -> Tot b) -> ib:b ->
+  HST.ST b
+    (requires (fun h0 -> B.live h0 buf))
+    (ensures (fun h0 v h1 -> 
+      h0 == h1 /\
+      v == fold_left_seq (B.as_seq h0 buf) f ib))
+    (decreases (B.length buf))
+let rec fold_left_buffer #a #b len buf f ib =
+  if len = 0ul then ib
+  else (fold_left_buffer (len - 1ul) (B.sub buf 1ul (len - 1ul)) 
+			 f (f ib (B.index buf 0ul)))
+
+val fold_left:
+  #a:Type -> #b:Type0 -> vec:vector a -> 
+  f:(b -> a -> Tot b) -> ib:b ->
+  HST.ST b
+    (requires (fun h0 -> live h0 vec))
+    (ensures (fun h0 v h1 ->
+      h0 == h1 /\
+      v == fold_left_seq (as_seq h0 vec) f ib))
+let fold_left #a #b vec f ib =
+  fold_left_buffer (Vec?.sz vec) (B.sub (Vec?.vs vec) 0ul (Vec?.sz vec)) f ib
+
+val forall_prop_seq:
+  #a:Type -> seq:S.seq a -> p:(a -> GTot Type0) -> GTot Type0
+let forall_prop_seq #a seq p =
+  forall (i:nat{i < S.length seq}). p (S.index seq i)
+
+val forall_prop_buffer:
+  #a:Type -> h:HS.mem -> buf:B.buffer a ->
+  p:(a -> GTot Type0) -> GTot Type0
+let forall_prop_buffer #a h buf p =
+  forall_prop_seq (B.as_seq h buf) p
+
+val forall_prop: 
+  #a:Type -> h:HS.mem -> vec:vector a -> 
+  p:(a -> Tot Type0) -> GTot Type0
+let forall_prop #a h vec p =
+  forall_prop_seq (as_seq h vec) p
+
+val forall_two_prop_seq:
+  #a:Type -> seq:S.seq a -> p:(a -> a -> GTot Type0) -> GTot Type0
+let forall_two_prop_seq #a seq p =
+  forall (i:nat{i < S.length seq}) (j:nat{j < S.length seq && i <> j}).
+    p (S.index seq i) (S.index seq j)
+
+val forall_two_prop_buffer:
+  #a:Type -> h:HS.mem -> buf:B.buffer a ->
+  p:(a -> a -> GTot Type0) -> GTot Type0
+let forall_two_prop_buffer #a h buf p =
+  forall_two_prop_seq (B.as_seq h buf) p
+
+val forall_two_prop:
+  #a:Type -> h:HS.mem -> vec:vector a -> 
+  p:(a -> a -> GTot Type0) -> GTot Type0
+let forall_two_prop #a h vec p =
+  forall_two_prop_seq (as_seq h vec) p
+
+
+(*! Facts *)
+
+val forall_prop_0:
+  #a:Type -> h:HS.mem -> vec:vector a{size_of vec = 0ul} ->
+  p:(a -> Tot Type0) ->
+  Lemma (forall_prop h vec p)
+let forall_prop_0 #a h vec p = ()
+
+val forall_prop_1:
+  #a:Type -> h:HS.mem -> vec:vector a{size_of vec = 1ul} ->
+  p:(a -> Tot Type0) ->
+  Lemma (forall_prop h vec p <==> p (S.index (as_seq h vec) 0))
+let forall_prop_1 #a h vec p = ()
+
+val forall_two_prop_0:
+  #a:Type -> h:HS.mem -> vec:vector a{size_of vec = 0ul} ->
+  p:(a -> a -> Tot Type0) ->
+  Lemma (forall_two_prop h vec p)
+let forall_two_prop_0 #a h vec p = ()
+
+val forall_two_prop_1:
+  #a:Type -> h:HS.mem -> vec:vector a{size_of vec = 1ul} ->
+  p:(a -> a -> Tot Type0) ->
+  Lemma (forall_two_prop h vec p)
+let forall_two_prop_1 #a h vec p = ()
+
+// val forall_prop_buffer_consistent:
+//   #a:Type -> h:HS.mem -> len:uint32_t{len > 0ul} ->
+//   buf:B.buffer a{B.len buf = len} ->
+//   vec:vector a ->
+//   p:(a -> Tot Type0) ->
+//   Lemma (requires (S.equal (as_seq h vec) (B.as_seq h buf) /\
+// 		  forall_prop_buffer h buf p))
+// 	(ensures (forall_prop h vec p))
+// let forall_prop_buffer_consistent #a h len buf vec p = ()
+
+// val forall_two_prop_buffer_consistent:
+//   #a:Type -> h:HS.mem -> len:uint32_t{len > 0ul} ->
+//   buf:B.buffer a{B.len buf = len} ->
+//   vec:vector a ->
+//   p:(a -> a -> Tot Type0) ->
+//   Lemma (requires (S.equal (as_seq h vec) (B.as_seq h buf) /\
+// 		  forall_two_prop_buffer h buf p))
+// 	(ensures (forall_two_prop h vec p))
+// let forall_two_prop_buffer_consistent #a h len buf vec p = ()
 
