examples/low-level/merkletree/MerkleTree.High.fst
@@ -20,46 +20,7 @@ let hash_seq = S.seq hash
 
 assume val hash_from_hashes: hash -> hash -> Tot hash
 
-/// About FStar.Seq.Base.seq (the library is not that rich enough..)
-
-val seq_map:
-  #a:Type -> #b:Type -> f:(a -> b) -> s:S.seq a -> 
-  Tot (fs:S.seq b{
-    S.length fs = S.length s /\
-    (forall (i:nat{i < S.length fs}). S.index fs i == f (S.index s i))})
-    (decreases (S.length s))
-let rec seq_map #a #b f s =
-  if S.length s = 0 then S.empty
-  else S.cons (f (S.head s)) (seq_map f (S.tail s))
-
-val seq_map_create:
-  #a:Type -> #b:Type -> f:(a -> b) -> 
-  len:nat -> ia:a ->
-  Lemma (seq_map f (S.create len ia) ==
-	S.create len (f ia))
-	[SMTPat (seq_map f (S.create len ia))]
-let rec seq_map_create #a #b f len ia =
-  S.lemma_eq_intro (seq_map f (S.create len ia)) (S.create len (f ia))
-
-val seq_map_append:
-  #a:Type -> #b:Type -> f:(a -> b) -> 
-  s1:S.seq a -> s2:S.seq a ->
-  Lemma (seq_map f (S.append s1 s2) ==
-	S.append (seq_map f s1) (seq_map f s2))
-	[SMTPat (seq_map f (S.append s1 s2))]
-let rec seq_map_append #a #b f s1 s2 =
-  S.lemma_eq_elim (seq_map f (S.append s1 s2)) 
-		  (S.append (seq_map f s1) (seq_map f s2))
-
-val seq_map_slice:
-  #a:Type -> #b:Type -> f:(a -> b) -> 
-  s:S.seq a -> i:nat -> j:nat{i <= j && j <= length s} ->
-  Lemma (seq_map f (S.slice s i j) == S.slice (seq_map f s) i j)
-	[SMTPat (seq_map f (S.slice s i j)); 
-	SMTPat (S.slice (seq_map f s) i j)]
-let seq_map_slice #a #b f s i j =
-  S.lemma_eq_elim (seq_map f (S.slice s i j))
-		  (S.slice (seq_map f s) i j)
+/// About FStar.Seq.Base.seq
 
 val lemma_split_append:
   #a:Type -> s1:S.seq a -> s2:S.seq a ->
