examples/low-level/merkletree/MerkleTree.Low.fst
@@ -1,6 +1,6 @@
 module MerkleTree.Low
 
-// TODO2: Use `EverCrypt.Hash` directly
+// TODO1: Use `EverCrypt.Hash` directly
 // open EverCrypt.Hash
 
 open FStar.All
@@ -11,36 +11,40 @@ open FStar.Seq
 open FStar.Integers
 open FStar.Ghost
 
+// TODO2: Connect high-level and low-level impls.
 open MerkleTree.High
-// TODO3: Use the vector library for hash values
-// open LowStar.Vector
+open LowStar.Vector
+open LowStar.BufVector
 
 module List = FStar.List.Tot
 module HS = FStar.HyperStack
 module HST = FStar.HyperStack.ST
+module MHS = FStar.Monotonic.HyperStack
+module HH = FStar.Monotonic.HyperHeap
+
 module B = LowStar.Buffer
-// module V = LowStar.Vector
+module V = LowStar.Vector
+module BV = LowStar.BufVector
 module S = FStar.Seq
 
 module High = MerkleTree.High
-
-let root = Monotonic.HyperHeap.root
 
 module U32 = FStar.UInt32
 module U8 = FStar.UInt8
 type uint32_t = U32.t
 type uint8_t = U8.t
 
-type hash = b:B.buffer uint8_t
-type vhash = h:hash{B.length h = hash_size}
-let hash_buf = B.buffer hash
+type hash = BV.lbuf uint8_t (UInt32.uint_to_t hash_size)
+let hash_vec = BV.buf_vector uint8_t (UInt32.uint_to_t hash_size)
 
-// TODO2: When `EverCrypt.Hash` is connected if we define it.
+// TODO1: When `EverCrypt.Hash` is connected if we define it.
 assume val hash_from_hashes: 
-  src1:vhash -> src2:vhash -> dst:vhash -> 
+  src1:hash -> src2:hash -> dst:hash -> 
   HST.ST unit
 	 (requires (fun h0 ->
-	   B.live h0 src1 /\ B.live h0 src2 /\ B.live h0 dst))
+	   B.live h0 src1 /\ not (B.g_is_null src1) /\
+	   B.live h0 src2 /\ not (B.g_is_null src2) /\
+	   B.live h0 dst /\ not (B.g_is_null dst)))
 	 (ensures (fun h0 _ h1 ->
 	   // memory safety
 	   modifies (loc_buffer dst) h0 h1 /\
@@ -48,6 +52,47 @@ assume val hash_from_hashes:
 	   High.hash_from_hashes 
 	     (B.as_seq h1 src1) 
 	     (B.as_seq h1 src2) = B.as_seq h1 dst)) 
+
+/// Sequence mapping
+
+val seq_map:
+  #a:Type -> #b:Type -> f:(a -> GTot b) -> s:S.seq a -> 
+  GTot (fs:S.seq b{
+    S.length fs = S.length s /\
+    (forall (i:nat{i < S.length fs}). S.index fs i == f (S.index s i))})
+    (decreases (S.length s))
+let rec seq_map #a #b f s =
+  if S.length s = 0 then S.empty
+  else S.cons (f (S.head s)) (seq_map f (S.tail s))
+
+val seq_map_create:
+  #a:Type -> #b:Type -> f:(a -> GTot b) -> 
+  len:nat -> ia:a ->
+  Lemma (seq_map f (S.create len ia) ==
+	S.create len (f ia))
+	[SMTPat (seq_map f (S.create len ia))]
+let rec seq_map_create #a #b f len ia =
+  S.lemma_eq_intro (seq_map f (S.create len ia)) (S.create len (f ia))
+
+val seq_map_append:
+  #a:Type -> #b:Type -> f:(a -> GTot b) -> 
+  s1:S.seq a -> s2:S.seq a ->
+  Lemma (seq_map f (S.append s1 s2) ==
+	S.append (seq_map f s1) (seq_map f s2))
+	[SMTPat (seq_map f (S.append s1 s2))]
+let rec seq_map_append #a #b f s1 s2 =
+  S.lemma_eq_elim (seq_map f (S.append s1 s2)) 
+		  (S.append (seq_map f s1) (seq_map f s2))
+
+val seq_map_slice:
+  #a:Type -> #b:Type -> f:(a -> GTot b) -> 
+  s:S.seq a -> i:nat -> j:nat{i <= j && j <= length s} ->
+  Lemma (seq_map f (S.slice s i j) == S.slice (seq_map f s) i j)
+	[SMTPat (seq_map f (S.slice s i j)); 
+	SMTPat (S.slice (seq_map f s) i j)]
+let seq_map_slice #a #b f s i j =
+  S.lemma_eq_elim (seq_map f (S.slice s i j))
+		  (S.slice (seq_map f s) i j)
 
 /// Utilities
 
@@ -110,449 +155,93 @@ val uint32_num_of_ones:
   n:uint32_t{U32.v n < pow2 (reveal sz)} ->
   Tot (nirs:uint32_t{U32.v nirs <= reveal sz /\ High.num_of_ones (U32.v n) = U32.v nirs})
       (decreases (U32.v n))
-#set-options "--z3rlimit 40"
 let rec uint32_num_of_ones sz n =
   if n = 0ul then 0ul
-  else (let nones = n % 2ul + uint32_num_of_ones (hide (reveal sz - 1)) (n / 2ul) in
-       assume (High.num_of_ones (U32.v n) = U32.v nones);
-       nones)
-
-/// About hash buffer
-
-val buffer_forall:
-  #a:Type -> h:HS.mem -> b:B.buffer a -> 
-  prop:(a -> GTot Type0) -> GTot Type0
-let buffer_forall #a h b prop =
-  forall (i:nat{i < B.length b}). prop (B.get h b i)
-
-val buffer_forall_gsub:
-  #a:Type -> h:HS.mem -> b:B.buffer a ->
-  prop:(a -> GTot Type0) ->
-  i:uint32_t -> len:uint32_t ->
-  Lemma (requires (U32.v i + U32.v len <= B.length b /\
-		  buffer_forall h b prop))
-	(ensures (buffer_forall h (B.gsub b i len) prop))
-let buffer_forall_gsub #a h b prop i len =
-  assert (forall (j:nat{j < B.length (B.gsub b i len)}).
-	 B.get h (B.gsub b i len) j == B.get h b (U32.v i + j))
-
-val buffer_forall_gsub_gsub:
-  #a:Type -> h:HS.mem -> b:B.buffer a ->
-  prop:(a -> GTot Type0) ->
-  i:uint32_t -> len:uint32_t ->
-  Lemma (requires (B.length b = U32.v len /\ i <= len /\
-		  buffer_forall h (B.gsub b 0ul i) prop /\
-		  buffer_forall h (B.gsub b i (len - i)) prop))
-	(ensures (buffer_forall h b prop))
-let buffer_forall_gsub_gsub #a h b prop i len =
-  assert (forall (j:nat{j < U32.v i}). B.get h b j == B.get h (B.gsub b 0ul i) j);
-  assert (forall (j:nat{j >= U32.v i && j < B.length b}).
-	 B.get h b j == B.get h (B.gsub b i (len - i)) (j - U32.v i))
-
-val hash_buf_allocated: 
-  h:HS.mem -> hs:hash_buf -> GTot Type0
-let hash_buf_allocated h hs =
-  buffer_forall h hs
-  (fun hb -> 
-    B.live h hb /\ 
-    B.length hb = hash_size /\ 
-    B.freeable hb)
-
-val hash_buf_allocated_gsub:
-  h:HS.mem -> hs:hash_buf ->
-  i:uint32_t -> len:uint32_t ->
-  Lemma (requires (U32.v i + U32.v len <= B.length hs /\
-		  hash_buf_allocated h hs))
-	(ensures (hash_buf_allocated h (B.gsub hs i len)))
-let hash_buf_allocated_gsub h hs i len =
-  buffer_forall_gsub h hs 
-  (fun hb -> B.live h hb /\ B.length hb = hash_size /\ B.freeable hb)
-  i len
-
-val hash_buf_allocated_gsub_gsub:
-  h:HS.mem -> hs:hash_buf ->
-  i:uint32_t -> len:uint32_t ->
-  Lemma (requires (B.length hs = U32.v len /\ i <= len /\
-		  hash_buf_allocated h (B.gsub hs 0ul i) /\
-		  hash_buf_allocated h (B.gsub hs i (len - i))))
-	(ensures (hash_buf_allocated h hs))
-	[SMTPat (hash_buf_allocated h (B.gsub hs 0ul i));
-	SMTPat (hash_buf_allocated h (B.gsub hs i (len - i)))]
-let hash_buf_allocated_gsub_gsub h hs i len =
-  buffer_forall_gsub_gsub h hs 
-  (fun hb -> B.live h hb /\ B.length hb = hash_size /\ B.freeable hb)
-  i len
-
-val hash_buf_allocated_gsub_hd_tl:
-  h:HS.mem -> hs:hash_buf ->
-  len:uint32_t{len > 0ul} ->
-  Lemma (requires (B.length hs = U32.v len /\
-		  B.live h (B.get h hs 0) /\ B.length (B.get h hs 0) = hash_size /\
-		  B.freeable (B.get h hs 0) /\
-		  hash_buf_allocated h (B.gsub hs 1ul (len - 1ul))))
-	(ensures (hash_buf_allocated h hs))
-	[SMTPat (hash_buf_allocated h (B.gsub hs 1ul (len - 1ul)))]
-let hash_buf_allocated_gsub_hd_tl h hs len =
-  buffer_forall_gsub_gsub h hs 
-  (fun hb -> B.live h hb /\ B.length hb = hash_size /\ B.freeable hb)
-  1ul len
-
-val loc_hashes: 
-  h:HS.mem -> hs:hash_buf -> 
-  GTot loc (decreases (B.length hs))
-let rec loc_hashes h hs =
-  if B.length hs = 0 then loc_none
-  else loc_union (loc_buffer (B.get h hs 0)) 
-		 (loc_hashes h (B.gsub hs 1ul (B.len hs - 1ul)))
-
-val loc_hashes_as_seq_eq:
-  hs:hash_buf -> h1:HS.mem -> h2:HS.mem ->
-  Lemma (requires (B.as_seq h1 hs == B.as_seq h2 hs))
-  	(ensures (loc_hashes h1 hs == loc_hashes h2 hs))
-	(decreases (B.length hs))
-	[SMTPat (B.as_seq h1 hs); SMTPat (B.as_seq h2 hs)]
-let rec loc_hashes_as_seq_eq hs h1 h2 =
-  if B.length hs = 0 then ()
-  else loc_hashes_as_seq_eq (B.gsub hs 1ul (B.len hs - 1ul)) h1 h2
-
-val loc_includes_union_left:
-  s1: loc -> s2: loc ->
-  Lemma (loc_includes (loc_union s1 s2) s1)
-let loc_includes_union_left s1 s2 =
-  loc_includes_union_l s1 s2 s1
-
-val loc_includes_union_right:
-  s1: loc -> s2: loc ->
-  Lemma (loc_includes (loc_union s1 s2) s2)
-let loc_includes_union_right s1 s2 =
-  loc_includes_union_l s1 s2 s2
-
-val loc_includes_union_lift_left:
-  s: loc -> s1: loc -> s2: loc ->
-  Lemma (requires (loc_includes s1 s2))
-	(ensures (loc_includes (loc_union s s1) (loc_union s s2)))
-let loc_includes_union_lift_left s s1 s2 =
-  loc_includes_union_left s s1;
-  loc_includes_union_right s s1;
-  loc_includes_union_r (loc_union s s1) s s2
-
-val loc_includes_union_lift_right:
-  s: loc -> s1: loc -> s2: loc ->
-  Lemma (requires (loc_includes s1 s2))
-	(ensures (loc_includes (loc_union s1 s) (loc_union s2 s)))
-let loc_includes_union_lift_right s s1 s2 =
-  loc_includes_union_left s1 s;
-  loc_includes_union_right s1 s;
-  loc_includes_union_r (loc_union s1 s) s s2
-
-val loc_hashes_gsub_includes':
-  h:HS.mem -> hs:hash_buf -> len:uint32_t ->
-  Lemma (requires (U32.v len <= B.length hs))
-	(ensures (loc_includes (loc_hashes h hs) 
-			       (loc_hashes h (B.gsub hs 0ul len))))
-	(decreases (B.length hs))
-let rec loc_hashes_gsub_includes' h hs len =
-  if len = 0ul then ()
-  else (loc_hashes_gsub_includes' h (B.gsub hs 1ul (B.len hs - 1ul)) (len - 1ul);
-       loc_includes_union_lift_left (loc_buffer (B.get h hs 0))
-				    (loc_hashes h (B.gsub hs 1ul (B.len hs - 1ul)))
-				    (loc_hashes h (B.gsub (B.gsub hs 0ul len) 1ul (len - 1ul))))
-
-val loc_hashes_gsub_includes:
-  h:HS.mem -> hs:hash_buf ->
-  i:uint32_t -> len:uint32_t ->
-  Lemma (requires (U32.v i + U32.v len <= B.length hs))
-	(ensures (loc_includes (loc_hashes h hs) 
-			       (loc_hashes h (B.gsub hs i len))))
-	(decreases (B.length hs))
-let rec loc_hashes_gsub_includes h hs i len =
-  if len = 0ul then ()
-  else if i = 0ul then loc_hashes_gsub_includes' h hs len
-  else (loc_hashes_gsub_includes h (B.gsub hs 1ul (B.len hs - 1ul)) (i - 1ul) len;
-       loc_includes_union_right (loc_buffer (B.get h hs 0))
-				(loc_hashes h (B.gsub hs 1ul (B.len hs - 1ul))))
-
-val hash_buf_disjoint_ext:
-  h:HS.mem -> hs:hash_buf -> 
-  #a:Type -> e:B.buffer a -> GTot Type0
-let hash_buf_disjoint_ext h hs #a e =
-  loc_disjoint (loc_hashes h hs) (loc_buffer e)
-
-val hash_buf_disjoint_ext_gsub:
-  h:HS.mem -> hs:hash_buf ->
-  i:uint32_t -> len:uint32_t ->
-  #a:Type -> e:B.buffer a ->
-  Lemma (requires (U32.v i + U32.v len <= B.length hs /\
-		  hash_buf_disjoint_ext h hs e))
-	(ensures (hash_buf_disjoint_ext h (B.gsub hs i len) e))
-let hash_buf_disjoint_ext_gsub h hs i len #a e =
-  loc_hashes_gsub_includes h hs i len
-
-val loc_hashes_gsub_gsub:
-  h:HS.mem -> hs:hash_buf -> i:uint32_t ->
-  Lemma (requires (U32.v i <= B.length hs))
-	(ensures (loc_hashes h hs ==
-		 loc_union (loc_hashes h (B.gsub hs 0ul i))
-			   (loc_hashes h (B.gsub hs i (B.len hs - i)))))
-	(decreases (U32.v i))
-#set-options "--z3rlimit 20"
-let rec loc_hashes_gsub_gsub h hs i =
-  if i = 0ul then ()
-  else (loc_hashes_gsub_gsub h (B.gsub hs 1ul (B.len hs - 1ul)) (i - 1ul);
-       loc_union_assoc
-	 (loc_buffer (B.get h hs 0))
-	 (loc_hashes h (B.gsub (B.gsub hs 1ul (B.len hs - 1ul)) 0ul (i - 1ul)))
-	 (loc_hashes h (B.gsub (B.gsub hs 1ul (B.len hs - 1ul)) (i - 1ul) (B.len hs - i))))
-
-val hash_buf_disjoint_ext_gsub_gsub:
-  h:HS.mem -> hs:hash_buf ->
-  i:uint32_t -> len:uint32_t ->
-  #a:Type -> e:B.buffer a ->
-  Lemma (requires (B.length hs = U32.v len /\ i <= len /\
-		  hash_buf_disjoint_ext h (B.gsub hs 0ul i) e /\
-		  hash_buf_disjoint_ext h (B.gsub hs i (len - i)) e))
-	(ensures (hash_buf_disjoint_ext h hs e))
-	[SMTPat (hash_buf_disjoint_ext h (B.gsub hs 0ul i) e);
-	SMTPat (hash_buf_disjoint_ext h (B.gsub hs i (len - i)) e)]
-let hash_buf_disjoint_ext_gsub_gsub h hs i len #a e =
-  loc_disjoint_union_r 
-    (loc_buffer e) 
-    (loc_hashes h (B.gsub hs 0ul i))
-    (loc_hashes h (B.gsub hs i (len - i)));
-  loc_hashes_gsub_gsub h hs i
-
-val hash_buf_disjoint:
-  h:HS.mem -> hs:hash_buf -> GTot Type0 (decreases (B.length hs))
-let rec hash_buf_disjoint h hs =
-// forall (i:nat{i < B.length hs}) (j:nat{j < B.length hs}).
-//   i <> j ==> (B.disjoint (B.get h hs i) (B.get h hs j))
-  if B.length hs = 0 then True
-  else (let ths = B.gsub hs 1ul (B.len hs - 1ul) in
-       loc_disjoint (loc_buffer (B.get h hs 0)) (loc_hashes h ths) /\
-       hash_buf_disjoint h ths)
+  else (admit ())
+  // let nones = n % 2ul + uint32_num_of_ones (hide (reveal sz - 1)) (n / 2ul) in
+  // assume (High.num_of_ones (U32.v n) = U32.v nones);
+  // nones)
 
 /// Low-level Merkle tree data structure
 
 noeq type merkle_tree =
-| MT: nelts:uint32_t ->
-      // The value buffer will be resized when elements are added.
-      // Resizing mechanism will be similar to that of C++ vector.
-      nvalues:uint32_t{nvalues >= nelts} ->
-      nvsz:erased nat{U32.v nvalues = pow2 (reveal nvsz) - 1} ->
-      values:hash_buf{B.length values = U32.v nvalues} ->
-      // The actual number of internal root values should be equal to 
-      // the number of "set" bits of `nelts`. The maximum number is
-      // U32.n (=32), so we pre-allocate the buffer.
-      iroots:hash_buf{B.length iroots = U32.n} ->
+| MT: values:hash_vec ->
+      iroots:hash_vec{V.size_of iroots = 32ul} ->
       merkle_tree
 
 let mt_ptr = B.pointer merkle_tree
 
-// val hashes_as_seq: HS.mem -> hash_buf -> GTot High.hash_seq
-val hashes_as_seq: 
-  h:HS.mem -> hb:hash_buf{hash_buf_allocated h hb} ->
-  GTot (hs:High.hash_seq{S.length hs = B.length hb})
-       (decreases (B.length hb))
-let rec hashes_as_seq h hb =
-  if B.length hb = 0 then S.empty
-  else (hash_buf_allocated_gsub h hb 1ul (B.len hb - 1ul);
-       S.cons (B.as_seq h (B.get h hb 0))
-	      (hashes_as_seq h (B.gsub hb 1ul (B.len hb - 1ul))))
-
-// val hashes_as_seq_gsub:
-//   h:HS.mem -> hb:hash_buf{hash_buf_allocated h hb} ->
-//   i:uint32_t ->
-//   len:uint32_t{U32.v i + U32.v len <= B.length hb} ->
-//   Lemma (ensures (hashes_as_seq h (B.gsub hb i len) =
-// 		 S.slice (hashes_as_seq h hb) (U32.v i) (U32.v i + U32.v len)))
-// 	(decreases (U32.v len))
-// 	[SMTPat (hashes_as_seq h hb); SMTPat (B.gsub hb i len)]
-// let rec hashes_as_seq_gsub h hb i len =
-//   // if len = 0ul then ()
-//   // else hashes_as_seq_gsub h hb (i + 1ul) (len - 1ul)
-//   admit ()
-
-// val hashes_as_seq_gsub_gsub:
-//   h:HS.mem -> hb:hash_buf{hash_buf_allocated h hb} ->
-//   len:uint32_t{U32.v len = B.length hb} ->
-//   i:uint32_t{i < len} ->
-//   Lemma (ensures (hashes_as_seq h hb =
-// 		 S.append (hashes_as_seq h (B.gsub hb 0ul i))
-// 			  (hashes_as_seq h (B.gsub hb i (len - i)))))
-// 	[SMTPat (hashes_as_seq h (B.gsub hb 0ul i));
-// 	SMTPat (hashes_as_seq h (B.gsub hb i (len - i)))]
-// let hashes_as_seq_gsub_gsub h hb len i =
-//   admit ()
-
 val merkle_tree_wf: HS.mem -> merkle_tree -> GTot Type0
 let merkle_tree_wf h mt =
-  let nelts = MT?.nelts mt in
-  let nirs = uint32_num_of_ones (hide 32) nelts in
-  let values = B.gsub (MT?.values mt) 0ul nelts in
-  let iroots = B.gsub (MT?.iroots mt) 0ul nirs in
-  hash_buf_allocated h values /\
-  hash_buf_allocated h iroots /\
-  iroots_of_hashes (hashes_as_seq h values) = hashes_as_seq h iroots
-
-val lift_mt: 
-  h:HS.mem -> mt:merkle_tree{merkle_tree_wf h mt} -> 
-  GTot High.merkle_tree
-let lift_mt h mt =
-  let nelts = MT?.nelts mt in
-  let nirs = uint32_num_of_ones (hide 32) nelts in
-  let values = hashes_as_seq h (B.gsub (MT?.values mt) 0ul nelts) in
-  let iroots = hashes_as_seq h (B.gsub (MT?.iroots mt) 0ul nirs) in
-  High.MT values iroots
+  // memory safety
+  BV.buf_vector_invariant h (MT?.values mt) /\
+  BV.buf_vector_invariant h (MT?.iroots mt) /\
+  V.frameOf (MT?.values mt) <> V.frameOf (MT?.iroots mt)
 
 /// Initialization
-
-// Allocate a buffer storing "pointers" to hashes.
-// The initial value for each pointer is null.
-val create_hashes:
-  len:uint32_t{len > 0ul} ->
-  HST.ST hash_buf
-	 (requires (fun h0 -> true))
-	 (ensures (fun h0 hs h1 ->
-	   B.unused_in hs h0 /\ B.live h1 hs /\
-	   B.length hs = U32.v len /\
-	   modifies loc_none h0 h1 /\
-	   B.freeable hs))
-let create_hashes len = 
-  B.malloc root B.null len
-
-val init_hashes: 
-  len:uint32_t -> hs:hash_buf{B.length hs = U32.v len} ->
-  HST.ST unit
-	 (requires (fun h0 -> B.live h0 hs))
-	 (ensures (fun h0 _ h1 ->
-	   hash_buf_allocated h1 hs /\
-	   B.live h1 hs /\ 
-	   modifies (loc_buffer hs) h0 h1))
-let rec init_hashes len hs =
-  if len = 0ul then ()
-  else (B.upd hs 0ul (B.malloc root (UInt8.uint_to_t 0) 32ul);
-       init_hashes (len - 1ul) (B.sub hs 1ul (len - 1ul));
-       let hh = HST.get () in
-       assert (hash_buf_allocated hh (B.gsub hs 0ul 1ul)))
-
-val init_hashes_partial:
-  idx:uint32_t -> len:uint32_t -> 
-  hs:hash_buf{U32.v idx + U32.v len <= B.length hs} ->
-  HST.ST unit
-	 (requires (fun h0 -> B.live h0 hs))
-	 (ensures (fun h0 _ h1 ->
-	   hash_buf_allocated h1 (B.gsub hs idx len) /\
-	   B.live h1 hs /\ 
-	   modifies (loc_buffer (B.gsub hs idx len)) h0 h1))
-let rec init_hashes_partial idx len hs =
-  init_hashes len (B.sub hs idx len)
 
 val create_merkle_tree: unit -> 
   HST.ST mt_ptr
 	 (requires (fun _ -> true))
 	 (ensures (fun h0 mt h1 ->
 	   merkle_tree_wf h1 (B.get h1 mt 0)))
-let create_merkle_tree _ = 
-  let values = B.null in
-  let iroots = create_hashes 32ul in
-  init_hashes 32ul iroots;
-  B.malloc root (MT 0ul 0ul (hide 0) values iroots) 1ul
+let create_merkle_tree _ =
+  let values = BV.create 1ul in
+  let iroots = BV.create 32ul in
+  // fresh_regions_neq (V.frameOf values) (V.frameOf iroots) hh0 hh1 hh2;
+  B.malloc root (MT values iroots) 1ul
 
 /// Insertion
 
-// NOTE: it DIRECTLY stores the `vs` pointer value (not copying the hash value).
-val insert_values:
-  mt:erased mt_ptr ->
-  nelts:uint32_t{U32.v nelts < UInt.max_int U32.n} ->
-  nvs:uint32_t{nvs >= nelts} ->
-  nvsz:erased nat{U32.v nvs = pow2 (reveal nvsz) - 1} ->  
-  vs:hash_buf{B.length vs = U32.v nvs} ->
-  e:vhash ->
-  HST.ST (ivs:hash_buf{B.length ivs = (if nelts = nvs then 2 * U32.v nelts + 1 else U32.v nvs)})
+// NOTE: it copies the value of `vs` buffer.
+val insert_value:
+  vs:hash_vec{not (V.is_full vs)} ->
+  rid:HH.rid{rid = V.frameOf vs} ->
+  nv:hash ->
+  HST.ST (ivs:hash_vec)
 	 (requires (fun h0 ->
-	   // hash_buf_allocated h0 (B.gsub vs 0ul nelts) /\
-	   B.live h0 e /\ B.freeable e /\ 
-	   B.live h0 vs /\ B.freeable vs /\
-	   B.live h0 (reveal mt) /\ B.disjoint (reveal mt) vs))
-	 (ensures (fun h0 ivs h1 ->
-	   // memory safety
-	   // hash_buf_allocated h1 (B.gsub ivs 0ul (nelts + 1ul)) /\
-	   B.live h1 ivs /\ B.freeable ivs /\
-	   modifies (loc_union (loc_buffer ivs) (loc_addr_of_buffer vs)) h0 h1 /\
-	   B.disjoint (reveal mt) ivs))
-	   // correctness
-	   // High.insert_values 
-	   //   (hashes_as_seq h0 (B.gsub vs 0ul nelts))
-	   //   (B.as_seq h0 e) =
-	   // hashes_as_seq h1 (B.gsub ivs 0ul (nelts + 1ul))))
-#set-options "--z3rlimit 20"
-let insert_values mt nelts nvs nvsz vs e =
-  if nelts = nvs
-  then (let hh0 = HST.get () in
-       pow2_lt_compat_inv (reveal nvsz) U32.n;
-       assert (2 * U32.v nelts + 1 <= UInt.max_int U32.n);
-       let ivs = create_hashes (2ul * nelts + 1ul) in
-       LowStar.BufferOps.blit vs 0ul ivs 0ul nelts;
-       B.upd ivs nelts e;
-       // init_hashes_partial nelts (nelts + 1ul) ivs;
-       B.free vs;
-       ivs)
-  else (B.upd vs nelts e;
-       // let hh0 = HST.get () in
-       // hash_buf_allocated_gsub_gsub hh0 (B.gsub vs 0ul (nelts + 1ul)) nelts (nelts + 1ul);
-       vs)
-
-val copy_hash: 
-  src:vhash -> dst:vhash -> 
-  HST.ST unit
-	 (requires (fun h0 -> 
-	   B.live h0 src /\ B.live h0 dst /\ B.disjoint src dst))
-	 (ensures (fun h0 _ h1 ->
-	   B.live h1 src /\ B.live h1 dst /\
-	   modifies (loc_buffer dst) h0 h1 /\
-	   B.as_seq h1 dst = B.as_seq h0 src))
-let copy_hash src dst =
-  blit src 0ul dst 0ul 32ul
+	   BV.buf_vector_invariant h0 vs /\
+	   B.live h0 nv /\ not (B.g_is_null nv)))
+	 (ensures (fun h0 ivs h1 -> 
+	   BV.buf_vector_invariant h1 ivs))
+let insert_value vs rid nv =
+  BV.insert_copy (UInt8.uint_to_t 0) vs rid nv
 
 val insert_iroots:
-  nirs:erased nat{reveal nirs <= U32.n} ->
-  nelts:uint32_t{U32.v nelts < pow2 (reveal nirs) - 1} ->
-  irs:hash_buf{B.length irs = reveal nirs} ->
-  nv:vhash ->
+  irs:hash_vec ->
+  nvalues:uint32_t{U32.v nvalues < pow2 (U32.v (V.size_of irs)) - 1} ->
+  nv:hash ->
   HST.ST unit
 	 (requires (fun h0 -> 
-	   B.live h0 irs /\ hash_buf_allocated h0 irs /\ B.live h0 nv /\ 
-	   B.disjoint irs nv /\ hash_buf_disjoint_ext h0 irs nv /\
-	   hash_buf_disjoint_ext h0 irs irs /\
-	   hash_buf_disjoint h0 irs))
-	 (ensures (fun h0 _ h1 -> 
-	   modifies (loc_hashes h0 irs) h0 h1 /\ // only affects internal root hash values
-	   hash_buf_allocated h1 irs)) // internal roots are still alive!
-#set-options "--z3rlimit 60"
-let rec insert_iroots nirs nelts irs nv =
-  let hh0 = HST.get () in
-  if nelts = 0ul
-  then copy_hash nv (B.index irs 0ul)
-  else (hash_buf_allocated_gsub hh0 irs 1ul (B.len irs - 1ul);
-       hash_buf_disjoint_ext_gsub hh0 irs 1ul (B.len irs - 1ul) nv;
-       hash_buf_disjoint_ext_gsub hh0 irs 1ul (B.len irs - 1ul) irs;
+	   BV.buf_vector_invariant h0 irs /\
+	   B.live h0 nv /\ not (B.g_is_null nv)))
+	 (ensures (fun h0 _ h1 ->
+	   BV.buf_vector_invariant h1 irs))
+let rec insert_iroots irs nvalues nv =
+  admit ()
+  // let hh0 = HST.get () in
+  // if nvalues = 0ul
+  // then copy_hash nv (B.index irs 0ul)
+  // else (hash_buf_allocated_gsub hh0 irs 1ul (B.len irs - 1ul);
+  //      hash_buf_disjoint_ext_gsub hh0 irs 1ul (B.len irs - 1ul) nv;
+  //      hash_buf_disjoint_ext_gsub hh0 irs 1ul (B.len irs - 1ul) irs;
        
-       insert_iroots (hide (reveal nirs - 1))
-		     (nelts - uint32_pow2 (uint32_pow2_floor nelts))
-		     (B.offset irs 1ul) nv;
+  //      insert_iroots (hide (reveal nirs - 1))
+  // 		     (nvalues - uint32_pow2 (uint32_pow2_floor nvalues))
+  // 		     (B.offset irs 1ul) nv;
 
-       let hh1 = HST.get () in
-       let tirs = B.offset irs 1ul in
-       B.modifies_buffer_elim (B.get hh1 irs 0) (loc_hashes hh1 tirs) hh0 hh1;
-       modifies_union_weakened_right (loc_buffer (B.get hh0 irs 0))
-       				     (loc_hashes hh0 tirs)
-       				     hh0 hh1);
-       Math.Lemmas.pow2_le_compat U32.n (reveal nirs);
+  //      let hh1 = HST.get () in
+  //      let tirs = B.offset irs 1ul in
+  //      B.modifies_buffer_elim (B.get hh1 irs 0) (loc_hashes hh1 tirs) hh0 hh1;
+  //      modifies_union_weakened_right (loc_buffer (B.get hh0 irs 0))
+  //      				     (loc_hashes hh0 tirs)
+  //      				     hh0 hh1);
+  //      Math.Lemmas.pow2_le_compat U32.n (reveal nirs);
 
-       if uint32_is_pow2 (nelts + 1ul)
-       then hash_from_hashes (B.index irs 0ul) (B.index irs 1ul)
-       	    		     (B.index irs 0ul)
-       else ()
+  //      if uint32_is_pow2 (nvalues + 1ul)
+  //      then hash_from_hashes (B.index irs 0ul) (B.index irs 1ul)
+  //      	    		     (B.index irs 0ul)
+  //      else ()
 
 val insert_maximum_helper:
   sz:nat -> n:uint32_t{U32.v n = pow2 sz - 1 && U32.v n < UInt.max_int U32.n} ->
@@ -561,168 +250,74 @@ let insert_maximum_helper sz n =
   pow2_lt_compat_inv sz U32.n
 
 val insert:
-  mt:mt_ptr -> e:vhash ->
+  mt:mt_ptr -> nv:hash ->
   HST.ST unit
 	 (requires (fun h0 -> 
-	   let mtv = B.get h0 mt 0 in
-	   let nelts = MT?.nelts mtv in
-	   let values = MT?.values mtv in
-	   let iroots = MT?.iroots mtv in
-
-	   U32.v nelts < UInt.max_int U32.n /\
-
-	   B.live h0 mt /\
-	   B.live h0 values /\
-	   B.freeable values /\
-	   // `B.disjoint mt values` should be better.
-	   loc_disjoint (loc_buffer mt) (loc_addr_of_buffer values) /\
-
-	   B.live h0 iroots /\
-	   hash_buf_allocated h0 iroots /\
-	   hash_buf_disjoint h0 iroots /\
-	   hash_buf_disjoint_ext h0 iroots iroots /\
-	   
-	   B.live h0 e /\ B.freeable e /\
-	   B.disjoint iroots e /\
-	   hash_buf_disjoint_ext h0 iroots e /\
-	   hash_buf_disjoint_ext h0 iroots values /\
-	   hash_buf_disjoint_ext h0 iroots mt))
-	 (ensures (fun h0 _ h1 -> true))
-let insert mt e =
+	   B.live h0 mt /\ not (B.g_is_null mt) /\
+	   (let mtv = B.get h0 mt 0 in
+	   merkle_tree_wf h0 mtv /\
+	   not (V.is_full (MT?.values mtv))) /\
+	   B.live h0 nv /\ not (B.g_is_null nv)))
+	 (ensures (fun h0 _ h1 ->
+	   merkle_tree_wf h1 (B.get h1 mt 0)))
+let insert mt nv =
   let mtv = B.index mt 0ul in
-  let nelts = MT?.nelts mtv in
   let values = MT?.values mtv in
-  let nvalues = MT?.nvalues mtv in
+  let nvalues = V.size_of values in
   let iroots = MT?.iroots mtv in
-  insert_iroots (hide 32) nelts iroots e;
-
-  let inelts = nelts + 1ul in
-  let invalues = 
-    if nelts = nvalues 
-    then (insert_maximum_helper (reveal (MT?.nvsz mtv)) nelts;
-	 2ul * nelts + 1ul)
-    else nvalues in
-  let invsz = hide (if nelts = nvalues then reveal (MT?.nvsz mtv) + 1 else reveal (MT?.nvsz mtv)) in
-  // let hh1 = HST.get () in assert (B.live hh1 mt);
-  let ivalues = insert_values (hide mt) nelts nvalues (MT?.nvsz mtv) values e in
-  loc_disjoint_union_r (loc_buffer mt)
-		       (loc_buffer ivalues)
-		       (loc_addr_of_buffer values);
-  // let hh2 = HST.get () in assert (B.live hh2 mt);
-  B.upd mt 0ul (MT inelts invalues invsz ivalues iroots)
+  insert_iroots iroots nvalues nv;
+  let ivalues = insert_value values (admit ()) nv in
+  admit (); B.upd mt 0ul (MT ivalues iroots)
 
 /// Getting the Merkle root
 
 val merkle_root_of_iroots:
-  nirs:uint32_t{U32.v nirs <= U32.n} ->
-  irs:hash_buf{B.length irs >= U32.v nirs} -> 
-  acc:vhash ->
+  irs:hash_vec ->
+  iidx:uint32_t{iidx < V.size_of irs} ->
+  acc:hash ->
   HST.ST unit
-	 (requires (fun h0 -> 
-	   B.live h0 irs /\ hash_buf_allocated h0 irs /\
-	   B.live h0 acc /\ B.disjoint irs acc))
-	 (ensures (fun h0 _ h1 -> 
-	   B.live h1 acc /\ modifies (loc_buffer acc) h0 h1))
-let rec merkle_root_of_iroots nirs irs acc =
-  if nirs = 0ul then ()
-  else (let hh0 = HST.get () in
-       hash_buf_allocated_gsub hh0 irs 1ul (nirs - 1ul);
-       assert (B.live hh0 (B.get hh0 irs 0));
-       merkle_root_of_iroots (nirs - 1ul) (B.sub irs 1ul (nirs - 1ul)) acc;
-       let hh1 = HST.get () in
-       assert (B.live hh1 (B.get hh1 irs 0));
-       hash_from_hashes (B.index irs 0ul) acc acc)
+	 (requires (fun h0 ->
+	   BV.buf_vector_invariant h0 irs /\
+	   B.live h0 acc /\ not (B.g_is_null acc)))
+	 (ensures (fun h0 _ h1 ->
+	   modifies (loc_buffer acc) h0 h1))
+let rec merkle_root_of_iroots irs iidx acc =
+  if iidx = 0ul 
+  then (admit (); hash_from_hashes (V.index irs 0ul) acc acc)
+  else (admit (); hash_from_hashes (V.index irs iidx) acc acc;
+       merkle_root_of_iroots irs (iidx - 1ul) acc)
 
 val get_root:
-  mt:mt_ptr -> rt:vhash ->
+  mt:mt_ptr -> rt:hash ->
   HST.ST unit
 	 (requires (fun h0 -> 
-	   B.live h0 mt /\ 
-	   B.live h0 (MT?.values (B.get h0 mt 0)) /\
-	   B.live h0 (MT?.iroots (B.get h0 mt 0)) /\
-	   hash_buf_allocated h0 (MT?.iroots (B.get h0 mt 0)) /\
-	   B.freeable (MT?.values (B.get h0 mt 0)) /\
-	   B.live h0 rt /\
-	   B.disjoint (MT?.iroots (B.get h0 mt 0)) rt))
-	 (ensures (fun h0 _ h1 -> true))
+	   B.live h0 mt /\ not (B.g_is_null mt) /\
+	   merkle_tree_wf h0 (B.get h0 mt 0) /\
+	   B.live h0 rt /\ not (B.g_is_null rt)))
+	 (ensures (fun h0 _ h1 ->
+	   modifies (loc_buffer rt) h0 h1))
 let get_root mt rt =
   let mtv = B.index mt 0ul in
-  let nelts = MT?.nelts mtv in
-  let irs = MT?.iroots mtv in
-  let nirs = uint32_num_of_ones (hide 32) nelts in
-  merkle_root_of_iroots nirs irs rt
+  let values = MT?.values mtv in
+  let nvalues = V.size_of values in
+  if nvalues = 0ul then ()
+  else (let iroots = MT?.iroots mtv in
+       let nirs = uint32_num_of_ones (hide 32) nvalues in
+       merkle_root_of_iroots iroots (nirs - 1ul) rt)
 
 /// Freeing the Merkle tree
-
-val free_hashes:
-  len:uint32_t ->
-  hs:hash_buf{B.length hs = U32.v len} ->
-  HST.ST unit
-	 (requires (fun h0 -> 
-	   B.live h0 hs /\ hash_buf_allocated h0 hs /\
-	   hash_buf_disjoint h0 hs /\
-	   hash_buf_disjoint_ext h0 hs hs))
-	 (ensures (fun h0 _ h1 -> modifies (loc_hashes h0 hs) h0 h1))
-	 (decreases (U32.v len))
-let rec free_hashes len hs = 
-  if len = 0ul then ()
-  else (let hh0 = HST.get () in
-       hash_buf_allocated_gsub hh0 hs 1ul (len - 1ul);
-       hash_buf_disjoint_ext_gsub hh0 hs 1ul (len - 1ul) hs;
-       free_hashes (len - 1ul) (B.sub hs 1ul (len - 1ul));
-
-       B.free (B.index hs 0ul);
-       
-       let hh1 = HST.get () in
-       assume (modifies (loc_hashes hh0 hs) hh0 hh1))
 
 val free_merkle_tree: 
   mt:mt_ptr ->
   HST.ST unit
 	 (requires (fun h0 -> 
-	   let mtv = B.get h0 mt 0 in
-	   let nelts = MT?.nelts mtv in
-	   let values = MT?.values mtv in
-	   let values_alloc = B.gsub values 0ul nelts in
-	   let iroots = MT?.iroots mtv in
-
-	   B.live h0 mt /\ B.freeable mt /\
-	   B.live h0 values /\ B.freeable values /\
-	   hash_buf_allocated h0 values_alloc /\
-	   hash_buf_disjoint h0 values_alloc /\
-	   hash_buf_disjoint_ext h0 values_alloc values /\
-	   hash_buf_disjoint_ext h0 values_alloc mt /\
-	   
-	   B.live h0 iroots /\ B.freeable iroots /\
-	   hash_buf_allocated h0 iroots /\
-	   hash_buf_disjoint h0 iroots /\
-	   hash_buf_disjoint_ext h0 iroots iroots /\
-	   hash_buf_disjoint_ext h0 iroots values /\
-	   hash_buf_disjoint_ext h0 iroots mt /\
-
-	   B.disjoint values iroots /\
-	   B.disjoint values mt /\
-	   B.disjoint iroots mt))
+	   B.live h0 mt /\ merkle_tree_wf h0 (B.get h0 mt 0)))
 	 (ensures (fun h0 _ h1 -> true))
-#set-options "--z3rlimit 40"
+	 // Should have sth. like: modifies (loc_mt mt) h0 h1
 let free_merkle_tree mt =
   let mtv = B.index mt 0ul in
-  let nelts = MT?.nelts mtv in
-  let values = MT?.values mtv in
-  let values_alloc = B.sub values 0ul nelts in
-  let iroots = MT?.iroots mtv in
-  free_hashes 32ul iroots;
-  B.free iroots;
-  
-  let hh0 = HST.get () in
-  assume (B.live hh0 values /\ B.freeable values /\
-  	 hash_buf_allocated hh0 values_alloc /\
-  	 hash_buf_disjoint hh0 values_alloc /\
-  	 hash_buf_disjoint_ext hh0 values_alloc values);
-  free_hashes nelts values_alloc;
-  B.free values;
-
-  let hh1 = HST.get () in 
-  assume (B.live hh1 mt /\ B.freeable mt);
+  admit ();
+  BV.free (MT?.values mtv);
+  BV.free (MT?.iroots mtv);
   B.free mt
 
