examples/low-level/merkletree/LowStar.BufVector.fst
@@ -1,0 +1,195 @@
+module LowStar.BufVector
+
+open FStar.All
+open FStar.Integers
+open LowStar.Modifies
+open LowStar.Vector
+
+module HH = FStar.Monotonic.HyperHeap
+module HS = FStar.HyperStack
+module HST = FStar.HyperStack.ST
+module MHS = FStar.Monotonic.HyperStack
+module S = FStar.Seq
+module B = LowStar.Buffer
+module V = LowStar.Vector
+
+type lbuf a (blen:uint32_t{blen > 0ul}) = 
+  b:B.buffer a{B.g_is_null b \/ B.len b = blen}
+type buf_vector a blen = V.vector (lbuf a blen)
+
+val new_region_:
+  r0:HH.rid -> 
+  HST.ST HH.rid
+    (fun _ -> HST.is_eternal_region r0)
+    (fun h0 r1 h1 ->
+      MHS.fresh_region r1 h0 h1 /\
+      HH.extends r1 r0 /\
+      HH.color r1 = HH.color r0 /\
+      HyperStack.ST.is_eternal_region r1 /\
+      modifies loc_none h0 h1)
+let new_region_ r0 =
+  let hh0 = HST.get () in
+  let r1 = HST.new_region r0 in
+  let hh1 = HST.get () in
+  B.modifies_none_modifies hh0 hh1;
+  r1
+
+type erid = rid:HH.rid{HST.is_eternal_region rid}
+
+val root: erid
+let root = HH.root
+
+/// The invariant
+
+val buf_vector_invariant_liveness:
+  #a:Type0 -> #blen:uint32_t{blen > 0ul} -> 
+  h:HS.mem -> bv:buf_vector a blen -> GTot Type0
+let buf_vector_invariant_liveness #a #blen h bv =
+  V.live h bv /\ V.freeable bv /\
+  V.forall_prop h bv 
+    (fun b -> B.live h b /\ (B.g_is_null b \/ B.freeable b))
+
+val buf_vector_invariant_region:
+  #a:Type0 -> #blen:uint32_t{blen > 0ul} -> 
+  h:HS.mem -> bv:buf_vector a blen -> GTot Type0
+let buf_vector_invariant_region #a #blen h bv =
+  HST.is_eternal_region (V.frameOf bv) /\
+  V.forall_prop h bv 
+    (fun b -> 
+      B.g_is_null b \/
+      (HH.extends (B.frameOf b) (V.frameOf bv) /\ 
+      B.frameOf b <> V.frameOf bv)) /\
+  V.forall_two_prop h bv
+    (fun b1 b2 -> 
+      B.g_is_null b1 \/ B.g_is_null b2 \/
+      B.frameOf b1 <> B.frameOf b2)
+
+val buf_vector_invariant:
+  #a:Type0 -> #blen:uint32_t{blen > 0ul} -> 
+  h:HS.mem -> bv:buf_vector a blen -> GTot Type0
+let buf_vector_invariant #a #blen h bv =
+  buf_vector_invariant_liveness h bv /\
+  buf_vector_invariant_region h bv
+
+val buf_vector_loc: 
+  #a:Type0 -> #blen:uint32_t{blen > 0ul} -> 
+  bv:buf_vector a blen -> GTot loc
+let buf_vector_loc #a #blen bv =
+  B.loc_regions false (FStar.Set.singleton (V.frameOf bv))
+
+/// Construction
+
+val create_rid:
+  #a:Type0 -> #blen:uint32_t{blen > 0ul} -> 
+  len:uint32_t{len > 0ul} -> rid:erid ->
+  HST.ST (buf_vector a blen)
+    (requires (fun h0 -> true))
+    (ensures (fun h0 bv h1 ->
+      buf_vector_invariant h1 bv /\
+      V.frameOf bv = rid /\
+      modifies loc_none h0 h1 /\
+      V.size_of bv = len))
+let create_rid #a #blen len rid =
+  V.create_rid len (B.null #a) rid
+
+val create:
+  #a:Type0 -> #blen:uint32_t{blen > 0ul} -> 
+  len:uint32_t{len > 0ul} ->
+  HST.ST (buf_vector a blen)
+    (requires (fun h0 -> true))
+    (ensures (fun h0 bv h1 ->
+      buf_vector_invariant h1 bv /\
+      MHS.fresh_region (V.frameOf bv) h0 h1 /\
+      modifies loc_none h0 h1 /\
+      V.size_of bv = len))
+let create #a #blen len =
+  let hh0 = HST.get () in
+  let nrid = new_region_ root in
+  let hh1 = HST.get () in
+  assert (MHS.fresh_region nrid hh0 hh1);
+  let bv = create_rid #a #blen len nrid in
+  let hh2 = HST.get () in
+  assume (MHS.fresh_region nrid hh0 hh2);
+  bv
+  
+// val assign:
+//   #a:Type -> #blen:uint32_t{blen > 0ul} ->
+//   bv:buf_vector a blen -> 
+//   i:uint32_t{i < V.size_of bv} -> v:lbuf a blen ->
+//   HST.ST unit
+//     (requires (fun h0 ->
+//       B.live h0 v /\ not (B.g_is_null v) /\
+//       buf_vector_invariant h0 bv))
+//     (ensures (fun h0 _ h1 -> 
+//       buf_vector_invariant h1 bv))
+// let assign #a #blen bv i v =
+//   let buf = V.index bv i in
+//   if B.is_null buf then
+//     admit () // V.assign bv i v
+//   else (assume (B.disjoint v buf);
+//        B.blit v 0ul buf 0ul blen)
+
+// insert_pointer: ...
+
+val insert_copy:
+  #a:Type0 -> ia:a -> #blen:uint32_t{blen > 0ul} ->
+  bv:buf_vector a blen{not (V.is_full bv)} ->
+  rid:HH.rid{rid = V.frameOf bv} ->
+  v:lbuf a blen ->
+  HST.ST (buf_vector a blen)
+    (requires (fun h0 -> 
+      B.live h0 v /\ not (B.g_is_null v) /\
+      buf_vector_invariant h0 bv))
+    (ensures (fun h0 ibv h1 -> 
+      buf_vector_invariant h1 ibv))
+let insert_copy #a ia #blen bv rid v =
+  let nrid = new_region_ rid in
+  let nv = B.malloc nrid ia blen in
+  B.blit v 0ul nv 0ul blen;
+  admit (); V.insert bv nv
+
+val assign_copy:
+  #a:Type0 -> ia:a -> #blen:uint32_t{blen > 0ul} ->
+  bv:buf_vector a blen ->
+  rid:HH.rid{rid = V.frameOf bv} ->
+  i:uint32_t{i < V.size_of bv} ->
+  v:lbuf a blen ->
+  HST.ST unit
+    (requires (fun h0 -> 
+      B.live h0 v /\ not (B.g_is_null v) /\
+      buf_vector_invariant h0 bv))
+    (ensures (fun h0 _ h1 -> 
+      buf_vector_invariant h1 bv))
+let assign_copy #a ia #blen bv rid i v =
+  let iv = V.index bv i in
+  if B.is_null iv 
+  then (let nrid = new_region_ rid in
+       let nv = B.malloc nrid ia blen in
+       B.blit v 0ul nv 0ul blen;
+       admit (); V.assign bv i nv)
+  else (admit (); B.blit v 0ul iv 0ul blen)
+
+val free_bufs:
+  #a:Type0 -> #blen:uint32_t{blen > 0ul} ->
+  bv:buf_vector a blen ->
+  idx:uint32_t{idx < V.size_of bv} ->
+  HST.ST unit
+    (requires (fun h0 -> buf_vector_invariant h0 bv))
+    (ensures (fun h0 _ h1 -> true))
+let rec free_bufs #a #blen bv idx =
+  admit ();
+  B.free (V.index bv idx);
+  if idx <> 0ul then
+    free_bufs bv (idx - 1ul)
+
+val free: 
+  #a:Type0 -> #blen:uint32_t{blen > 0ul} ->
+  bv:buf_vector a blen ->
+  HST.ST unit
+    (requires (fun h0 -> buf_vector_invariant h0 bv))
+    (ensures (fun h0 _ h1 -> modifies (buf_vector_loc bv) h0 h1))
+let free #a #blen bv =
+  (if V.size_of bv = 0ul then () else free_bufs bv (V.size_of bv - 1ul));
+  admit ();
+  V.free bv
+
